---
output:
  html_document:
    css: style1.css
    theme: cosmo
    highlight: textmate
---

## Formulario Econometría {.tabset .tabset-pills}

### Modelo Univariado


$$y_i=\beta_0+\beta_1x_{1,i}+u_i$$
Bajo los supuestos de regresión lineal

$$\hat{\beta_o}=\overline{y}-\hat{\beta_1} \overline{x_{1}}$$
$$\hat{\beta_1}=\frac{\sum_{i=1}^{T} (x_{1,i}-\overline{x_{1}})(y_i-\overline{y})}{\sum_{i=1}^{T} (x_{1,i}-\overline{x_{1}})^2}=\frac{\sum_{i=1}^{T} (x_{1,i}-\overline{x_1})y_i}{\sum_{i=1}^{T} (x_{1,i}-\overline{x_1})^2}=\frac{\sum_{i=1}^{T} (y_i-\overline{y})x_{1,i}}{\sum_{i=1}^{T} (x_{1,i}-\overline{x_{1}})^2}$$

$$\hat{y_i}=\hat{\beta_0}+\hat{\beta_1}x_{1.i}$$
$$\hat{u_i}=y_i-\hat{y_i}$$

$$\mathbb{E} [\hat{\beta_0}]=\beta_0$$
$$\mathbb{E} [\hat{\beta_1}]=\beta_1$$

$$Var(\hat{\beta_0})=\frac{\sigma^2 \sum_{i=1}^T x_{1,i}^2}{T \cdot \sum_{i=1}^T (x_{1,i}-\overline{x_1})^2}=\frac{\sigma^2 \sum_{i=1}^T x_{1,i}^2}{T \cdot SST_1}$$
$$Var(\hat{\beta_1})=\frac{\sigma^2}{\sum_{i=1}^T (x_{1.i}-\overline{x_1})}=\frac{\sigma^2}{SST_1}$$

$$\hat{\sigma}^2=\frac{\sum_{i=1}^T \hat{u_i} }{T-K-1}$$

### $R^2$

$$SST=SSE+SSR$$

$$\sum_{i=1}^{T} (y_i-\overline{y})^2 = \sum_{i=1}^{T} (\hat{y_i}-\overline{y})^2 + \sum_{i=1}^{T} (y_i-\hat{y_i})^2$$

$$R^2=\frac{\sum_{i=1}^{T} (\hat{y_i}-\overline{y})^2}{\sum_{i=1}^{T} (y_i-\overline{y})^2}=1-\frac{\sum_{i=1}^{T} (y_i-\hat{y_i})^2}{\sum_{i=1}^{T} (y_i-\overline{y})^2}$$

### Modelo Multivariado

$$y_i=\beta_0+\beta_1x_{1,i}+\beta_2x_{2,i}+...+\beta_kx_{k,i}+u_i$$

Bajo los supuestos de regresión lineal 

$$\mathbb{E} [\hat{\beta_j}]=\beta_j$$
$$Var(\hat{\beta_j})=\frac{\sigma^2}{SST_j(1-R_j^2)}=\frac{\sigma^2}{SST_j}\cdot VIF_j$$


| Modelos 	| Regresión 	| $\beta_1$ 	| $Pendiente=\frac{\partial y}{\partial x}$ 	| Interpretación 	|
|:---:	|:---:	|:---:	|:---:	|:---:	|
| Nivel-Nivel 	| $y_i=\beta_0+\beta_1x_i+u_i$ 	| $\frac{\Delta y_i}{\Delta x_i}$ 	| $\beta_1$ 	| Cambio en nivel 	|
| Nivel-Log 	| $y_i=\beta_0+\beta_1 ln(x_i)+u_i$ 	| $\frac{\Delta y_i}{\Delta \%x_i}$ 	| $\beta_1 \frac{1}{x}$ 	| Semi-Elasticidad 	|
| Log-Nivel 	| $ln(y_i)=\beta_0+\beta_1x_i+u_i$ 	| $\frac{\Delta \%y_i}{\Delta x_i}$ 	| $\beta_1 y$ 	| Semi-Elasticidad 	|
| Log-Log 	| $ln(y_i)=\beta_0+\beta_1 ln(x_i)+u_i$ 	| $\frac{\Delta \%y_i}{\Delta \%x_i}$ 	| $\beta_1 \frac{y}{x}$ 	| Elasticidad 	|


### Sesgo

$$y_i=\beta_0+\beta_1x_{1,i}+\beta_1x_{2,i}+u_i \Rightarrow Real$$
$$y_i=\gamma_0+\gamma_1x_{1,i}+u_i \Rightarrow Estimado$$


$$\mathbb{E}[\hat{\gamma_1}]=\beta_1+\underbrace{\beta_2 \frac{Cov(X_1,X_2)}{Var(X_1)}}_{\text Sesgo}$$

|  	| $Cov(X_1,X_2)>0$ 	| $Cov(X_1,X_2)<0$ 	|
|:---:	|:---:	|:---:	|
| $\beta_2>0$ 	| Sobrevalorado 	| Subvalorado 	|
| $\beta_2<0$ 	| Subvalorado 	| Sobrevalorado 	|



### Inferencia

$$t_{\hat{\beta_j}}= \frac{\hat{\beta_j}-\beta_j}{sd(\hat{\beta_j})} \sim t_{(T-K-1)}$$

$$Pr\left[ \hat{\beta_j}-c_{\alpha} \cdot sd(\hat{\beta_j}) < \hat{\beta_j} <\hat{\beta_j}+c_{\alpha} \cdot sd(\hat{\beta_j})\right]=1-\alpha$$

$$P_{value}=Pr[|t_{\hat{\beta_j}}|\geq |t_{obs}|]$$

$$F_{obs}=\frac{(SSR_{r}-SSR_{ur})/q}{(SSR_{ur})/(T-K-1)}=\frac{(R_{ur}^2-R_{r}^2)/q}{(1-R_{ur}^2)/(T-K-1)} \sim F_{q, t-k-1}$$

